# baseURI: https://w3id.org/con-tax/properties/bhp
# prefix: bhp

@prefix : <https://w3id.org/con-tax/properties/bhp#> .
@prefix aat: <http://vocab.getty.edu/aat/> .
@prefix bhp: <https://w3id.org/con-tax/properties/bhp#> .
@prefix bot: <https://w3id.org/bot#> .
@prefix cc: <http://creativecommons.org/ns#> .
@prefix contax: <https://w3id.org/con-tax#> .
@prefix cp: <https://w3id.org/con-tax/properties/cp#> .
@prefix dbr: <http://dbpedia.org/resource/> .
@prefix dct: <http://purl.org/dc/terms/> .
@prefix dcterms: <http://purl.org/dc/terms/> .
@prefix gvp: <http://vocab.getty.edu/ontology#> .
@prefix iso-thes: <http://purl.org/iso25964/skos-thes#> .
@prefix owl: <http://www.w3.org/2002/07/owl#> .
@prefix rdf: <http://www.w3.org/1999/02/22-rdf-syntax-ns#> .
@prefix rdfs: <http://www.w3.org/2000/01/rdf-schema#> .
@prefix schema: <http://schema.org/> .
@prefix skos: <http://www.w3.org/2004/02/skos/core#> .
@prefix vann: <http://purl.org/vocab/vann/> .
@prefix vcard: <http://www.w3.org/2006/vcard/ns#> .
@prefix voaf: <http://purl.org/vocommons/voaf#> .
@prefix wd: <http://www.wikidata.org/entity/> .
@prefix xl: <http://www.w3.org/2008/05/skos-xl#> .
@prefix xsd: <http://www.w3.org/2001/XMLSchema#> .

<http://pi.pauwel.be/voc/buildingelement#Slab-ROOF>
  rdf:type rdfs:Resource ;
.
dcterms:source
  rdf:type rdf:Property ;
.
<http://w3id.org/con-tax/zones/et-buildings#319>
  rdf:type rdfs:Resource ;
.
<http://w3id.org/con-tax/zones/et-buildings#321>
  rdf:type rdfs:Resource ;
.
<http://w3id.org/con-tax/zones/et-buildings#323>
  rdf:type rdfs:Resource ;
.
<http://w3id.org/con-tax/zones/et-buildings#359>
  rdf:type rdfs:Resource ;
.
<http://w3id.org/con-tax/zones/et-buildings#466>
  rdf:type rdfs:Resource ;
.
<http://w3id.org/con-tax/zones/et-buildings#520>
  rdf:type rdfs:Resource ;
.
<http://w3id.org/con-tax/zones/et-buildings#63>
  rdf:type rdfs:Resource ;
.
<http://w3id.org/con-tax/zones/et-buildings293>
  rdf:type rdfs:Resource ;
.
vcard:Individual
  rdf:type rdfs:Resource ;
.
vcard:Organization
  rdf:type rdfs:Resource ;
.
<https://id.erfgoed.net/thesauri/aanduidingstypes>
  rdf:type rdfs:Resource ;
.
<https://id.erfgoed.net/thesauri/dateringen/1195>
  rdf:type rdfs:Resource ;
.
<https://id.erfgoed.net/thesauri/dateringen/1196>
  rdf:type rdfs:Resource ;
.
<https://id.erfgoed.net/thesauri/dateringen/1223>
  rdf:type rdfs:Resource ;
.
<https://id.erfgoed.net/thesauri/dateringen/1227>
  rdf:type rdfs:Resource ;
.
<https://id.erfgoed.net/thesauri/dateringen/1236>
  rdf:type rdfs:Resource ;
.
<https://id.erfgoed.net/thesauri/dateringen/1237>
  rdf:type rdfs:Resource ;
.
<https://id.erfgoed.net/thesauri/waardetypes>
  rdf:type rdfs:Resource ;
.
<https://id.erfgoed.net/thesauri/waardetypes/30>
  rdf:type skos:Concept ;
.
<https://id.erfgoed.net/thesauri/waardetypes/37>
  rdf:type skos:Concept ;
.
<https://inventaris.onroerenderfgoed.be/>
  rdf:type rdfs:Resource ;
.
bot:Building
  rdf:type owl:Class ;
.
bot:Element
  rdf:type owl:Class ;
.
bot:Interface
  rdf:type owl:Class ;
.
bot:Site
  rdf:type owl:Class ;
.
bot:Zone
  rdf:type owl:Class ;
.
contax:Architect
  rdf:type owl:Class ;
.
contax:ConstructionComponent
  rdf:type owl:Class ;
.
contax:Material
  rdf:type owl:Class ;
.
contax:domainOrSubjectIncludes
  rdf:type owl:AnnotationProperty ;
.
contax:property_DP
  rdf:type owl:DatatypeProperty ;
.
contax:property_OP
  rdf:type owl:ObjectProperty ;
.
contax:rangeOrObjectIncludes
  rdf:type owl:AnnotationProperty ;
.
<https://w3id.org/con-tax/components/aat-arch#300002098>
  rdf:type rdfs:Resource ;
.
<https://w3id.org/con-tax/properties/bhp>
  rdf:type voaf:Vocabulary ;
  rdf:type owl:Ontology ;
  cc:license <https://creativecommons.org/licenses/by/4.0/> ;
  dcterms:creator [
      rdf:type vcard:Individual ;
      vcard:family-name "Bonduel" ;
      vcard:fn "Mathias Bonduel" ;
      vcard:given-name "Mathias" ;
      vcard:hasOrganizationName [
          rdf:type vcard:Organization ;
          owl:sameAs dbr:Katholieke_Universiteit_Leuven ;
          vcard:hasURL <https://www.kuleuven.be> ;
          vcard:organization-name "KU Leuven" ;
        ] ;
      vcard:hasURL <https://orcid.org/0000-0002-3313-924X> ;
      vcard:hasURL <https://www.kuleuven.be/wieiswie/nl/person/00110827> ;
      vcard:hasURL <https://www.researchgate.net/profile/Mathias_Bonduel> ;
    ] ;
  dcterms:description "This ontology contains a preliminary list of properties that might prove useful to describe heritage buildings. The properties are inspired by (1) the databases of Monumentenwacht Vlaanderen (MAKSBO and IMACS), (2) the online built heritage inventory of Onroerend Erfgoed Vlaanderen and (3) the results of interviews with a large variety of Flemish built heritage stakeholders."@en ;
  dcterms:issued "2020-11-30"^^xsd:date ;
  dcterms:title "Built Heritage Properties (BHP) taxonomy"@en ;
  vann:preferredNamespacePrefix "bhp" ;
  vann:preferredNamespaceUri "https://w3id.org/con-tax/properties/bhp#" ;
  rdfs:comment "- Version 0.0.1: initial version"@en ;
  owl:versionInfo "0.0.1" ;
.
bhp:buildingFunction
  rdf:type owl:ObjectProperty ;
  dcterms:source <https://www.monumentenwacht.be/> ;
  rdfs:comment "Property to assign a function to a certain built heritage building. For the Flemish context, predefined property values can be used from ET-BUILDINGS taxonomy, based on the Onroerend Erfgoed thesaurus \"ERFGOEDTYPES\", and the AAT-BUILDINGS taxonomy based on the Getty AAT. Property definition inspired by the Monumentenwacht Vlaanderen databases (MAKSBO and IMACS)."@en ;
  rdfs:isDefinedBy <https://w3id.org/con-tax/properties/bhp> ;
  rdfs:label "building function"@en ;
  rdfs:subPropertyOf contax:property_OP ;
  contax:domainOrSubjectIncludes bot:Building ;
  contax:rangeOrObjectIncludes <http://w3id.org/con-tax/zones/et-buildings#1226> ;
  contax:rangeOrObjectIncludes <http://w3id.org/con-tax/zones/et-buildings#1271> ;
  contax:rangeOrObjectIncludes <http://w3id.org/con-tax/zones/et-buildings#293> ;
  contax:rangeOrObjectIncludes <http://w3id.org/con-tax/zones/et-buildings#319> ;
  contax:rangeOrObjectIncludes <http://w3id.org/con-tax/zones/et-buildings#321> ;
  contax:rangeOrObjectIncludes <http://w3id.org/con-tax/zones/et-buildings#323> ;
  contax:rangeOrObjectIncludes <http://w3id.org/con-tax/zones/et-buildings#359> ;
  contax:rangeOrObjectIncludes <http://w3id.org/con-tax/zones/et-buildings#466> ;
  contax:rangeOrObjectIncludes <http://w3id.org/con-tax/zones/et-buildings#520> ;
  contax:rangeOrObjectIncludes <http://w3id.org/con-tax/zones/et-buildings#63> ;
  contax:rangeOrObjectIncludes <https://w3id.org/con-tax/zones/aat-buildings#300004790> ;
.
bhp:buildingFunction_current
  rdf:type owl:ObjectProperty ;
  dcterms:source <https://www.monumentenwacht.be/> ;
  rdfs:comment "Property to assign a current function to a certain built heritage building. An alternative way of modeling the current function of a building is by attaching the appropriate class (specialization of bot:Building) to the building node via an rdf:type relation. For the Flemish context, predefined property values can be used from ET-BUILDINGS taxonomy, based on the Onroerend Erfgoed thesaurus \"ERFGOEDTYPES\", and the AAT-BUILDINGS taxonomy based on the Getty AAT. Property definition inspired by the Monumentenwacht Vlaanderen databases (MAKSBO and IMACS)."@en ;
  rdfs:isDefinedBy <https://w3id.org/con-tax/properties/bhp> ;
  rdfs:label "current building function"@en ;
  rdfs:subPropertyOf bhp:buildingFunction ;
  contax:domainOrSubjectIncludes bot:Building ;
  contax:rangeOrObjectIncludes <http://w3id.org/con-tax/zones/et-buildings#1226> ;
  contax:rangeOrObjectIncludes <http://w3id.org/con-tax/zones/et-buildings#1271> ;
  contax:rangeOrObjectIncludes <http://w3id.org/con-tax/zones/et-buildings#293> ;
  contax:rangeOrObjectIncludes <http://w3id.org/con-tax/zones/et-buildings#319> ;
  contax:rangeOrObjectIncludes <http://w3id.org/con-tax/zones/et-buildings#321> ;
  contax:rangeOrObjectIncludes <http://w3id.org/con-tax/zones/et-buildings#323> ;
  contax:rangeOrObjectIncludes <http://w3id.org/con-tax/zones/et-buildings#359> ;
  contax:rangeOrObjectIncludes <http://w3id.org/con-tax/zones/et-buildings#466> ;
  contax:rangeOrObjectIncludes <http://w3id.org/con-tax/zones/et-buildings#520> ;
  contax:rangeOrObjectIncludes <http://w3id.org/con-tax/zones/et-buildings#63> ;
  contax:rangeOrObjectIncludes <https://w3id.org/con-tax/zones/aat-buildings#300004790> ;
.
bhp:buildingFunction_original
  rdf:type owl:ObjectProperty ;
  dcterms:source <https://www.monumentenwacht.be/> ;
  rdfs:comment "Property to assign an original function to a certain built heritage building. For the Flemish context, predefined property values can be used from ET-BUILDINGS taxonomy, based on the Onroerend Erfgoed thesaurus \"ERFGOEDTYPES\", and the AAT-BUILDINGS taxonomy based on the Getty AAT. Property definition inspired by the Monumentenwacht Vlaanderen databases (MAKSBO and IMACS)."@en ;
  rdfs:isDefinedBy <https://w3id.org/con-tax/properties/bhp> ;
  rdfs:label "original building function"@en ;
  rdfs:subPropertyOf bhp:buildingFunction ;
  contax:domainOrSubjectIncludes bot:Building ;
  contax:rangeOrObjectIncludes <http://w3id.org/con-tax/zones/et-buildings#1226> ;
  contax:rangeOrObjectIncludes <http://w3id.org/con-tax/zones/et-buildings#1271> ;
  contax:rangeOrObjectIncludes <http://w3id.org/con-tax/zones/et-buildings#293> ;
  contax:rangeOrObjectIncludes <http://w3id.org/con-tax/zones/et-buildings#319> ;
  contax:rangeOrObjectIncludes <http://w3id.org/con-tax/zones/et-buildings#321> ;
  contax:rangeOrObjectIncludes <http://w3id.org/con-tax/zones/et-buildings#323> ;
  contax:rangeOrObjectIncludes <http://w3id.org/con-tax/zones/et-buildings#359> ;
  contax:rangeOrObjectIncludes <http://w3id.org/con-tax/zones/et-buildings#466> ;
  contax:rangeOrObjectIncludes <http://w3id.org/con-tax/zones/et-buildings#520> ;
  contax:rangeOrObjectIncludes <http://w3id.org/con-tax/zones/et-buildings#63> ;
  contax:rangeOrObjectIncludes <https://w3id.org/con-tax/zones/aat-buildings#300004790> ;
.
bhp:buildingFunction_past
  rdf:type owl:ObjectProperty ;
  dcterms:source <https://www.monumentenwacht.be/> ;
  rdfs:comment "Property to assign a past function (different from the original function) to a certain built heritage building. For the Flemish context, predefined property values can be used from ET-BUILDINGS taxonomy, based on the Onroerend Erfgoed thesaurus \"ERFGOEDTYPES\", and the AAT-BUILDINGS taxonomy based on the Getty AAT. Property definition inspired by the Monumentenwacht Vlaanderen databases (MAKSBO and IMACS)."@en ;
  rdfs:isDefinedBy <https://w3id.org/con-tax/properties/bhp> ;
  rdfs:label "past building function"@en ;
  rdfs:subPropertyOf bhp:buildingFunction ;
  contax:domainOrSubjectIncludes bot:Building ;
  contax:rangeOrObjectIncludes <http://w3id.org/con-tax/zones/et-buildings#1226> ;
  contax:rangeOrObjectIncludes <http://w3id.org/con-tax/zones/et-buildings#1271> ;
  contax:rangeOrObjectIncludes <http://w3id.org/con-tax/zones/et-buildings#293> ;
  contax:rangeOrObjectIncludes <http://w3id.org/con-tax/zones/et-buildings#319> ;
  contax:rangeOrObjectIncludes <http://w3id.org/con-tax/zones/et-buildings#321> ;
  contax:rangeOrObjectIncludes <http://w3id.org/con-tax/zones/et-buildings#323> ;
  contax:rangeOrObjectIncludes <http://w3id.org/con-tax/zones/et-buildings#359> ;
  contax:rangeOrObjectIncludes <http://w3id.org/con-tax/zones/et-buildings#466> ;
  contax:rangeOrObjectIncludes <http://w3id.org/con-tax/zones/et-buildings#520> ;
  contax:rangeOrObjectIncludes <http://w3id.org/con-tax/zones/et-buildings#63> ;
  contax:rangeOrObjectIncludes <https://w3id.org/con-tax/zones/aat-buildings#300004790> ;
.
bhp:describedByHistoricalSource
  rdf:type owl:ObjectProperty ;
  rdfs:comment "A property to connect a spatial building zone or construction component to a historical source that describes it. Property definition inspired by interviews with built heritage stakeholders."@en ;
  rdfs:isDefinedBy <https://w3id.org/con-tax/properties/bhp> ;
  rdfs:label "described by historical source"@en ;
  rdfs:subPropertyOf contax:property_OP ;
  contax:domainOrSubjectIncludes bot:Element ;
  contax:domainOrSubjectIncludes bot:Zone ;
  contax:domainOrSubjectIncludes contax:ConstructionComponent ;
.
bhp:hasArchitecturalStyle
  rdf:type owl:ObjectProperty ;
  rdfs:comment "Property to indicate the architectural style of as spatial building zone or a construction component. Property definition inspired by interviews with built heritage stakeholders."@en ;
  rdfs:isDefinedBy <https://w3id.org/con-tax/properties/bhp> ;
  rdfs:label "has architectural style"@en ;
  rdfs:subPropertyOf contax:property_OP ;
  contax:domainOrSubjectIncludes bot:Element ;
  contax:domainOrSubjectIncludes bot:Zone ;
  contax:domainOrSubjectIncludes contax:ConstructionComponent ;
.
bhp:hasErfgoedBeheersplan
  rdf:type owl:ObjectProperty ;
  rdfs:comment "Property to connect a built heritage buildig or site to an \"erfgoed beheersplan\", as defined by Onroerend Erfgoed Vlaanderen. Property definition inspired by interviews with built heritage stakeholders."@en ;
  rdfs:isDefinedBy <https://w3id.org/con-tax/properties/bhp> ;
  rdfs:label "has erfgoed beheersplan"@en ;
  rdfs:subPropertyOf contax:property_OP ;
  contax:domainOrSubjectIncludes bot:Building ;
  contax:domainOrSubjectIncludes bot:Site ;
.
bhp:heritageProtectionType
  rdf:type owl:ObjectProperty ;
  dcterms:source <https://inventaris.onroerenderfgoed.be/> ;
  rdfs:comment "Property to assign a heritage protection type to a certain built heritage site or building. For the Flemish context, two predefined property values can be used from the Onroerend Erfgoed thesaurus \"AANDUIDINGSTYPES\". Property definition inspired by the Onroerend Erfgoed Vlaanderen built heritage inventory."@en ;
  rdfs:isDefinedBy <https://w3id.org/con-tax/properties/bhp> ;
  rdfs:label "heritage protection type"@en ;
  rdfs:subPropertyOf contax:property_OP ;
  contax:domainOrSubjectIncludes bot:Building ;
  contax:domainOrSubjectIncludes bot:Site ;
  contax:rangeOrObjectIncludes <https://id.erfgoed.net/thesauri/aanduidingstypes/1> ;
  contax:rangeOrObjectIncludes <https://id.erfgoed.net/thesauri/aanduidingstypes/9> ;
.
bhp:heritageValue
  rdf:type owl:ObjectProperty ;
  dcterms:source <https://inventaris.onroerenderfgoed.be/> ;
  rdfs:comment "Property to assign a heritage value to a certain built heritage object (spatial building zone or individual construction component). For the Flemish context, predefined property values can be used from the Onroerend Erfgoed thesaurus \"WAARDETYPES\". Property definition inspired by the Onroerend Erfgoed Vlaanderen built heritage inventory."@en ;
  rdfs:isDefinedBy <https://w3id.org/con-tax/properties/bhp> ;
  rdfs:label "heritage value"@en ;
  rdfs:subPropertyOf contax:property_OP ;
  contax:domainOrSubjectIncludes bot:Element ;
  contax:domainOrSubjectIncludes bot:Zone ;
  contax:domainOrSubjectIncludes contax:ConstructionComponent ;
  contax:rangeOrObjectIncludes <https://id.erfgoed.net/thesauri/waardetypes/30> ;
  contax:rangeOrObjectIncludes <https://id.erfgoed.net/thesauri/waardetypes/37> ;
.
bhp:locationOfHistoricalEvent
  rdf:type owl:ObjectProperty ;
  rdfs:comment "A property to connect a spatial building zone to a historical event that took place in the building zone. Property definition inspired by interviews with built heritage stakeholders."@en ;
  rdfs:isDefinedBy <https://w3id.org/con-tax/properties/bhp> ;
  rdfs:label "location of historical event"@en ;
  rdfs:subPropertyOf contax:property_OP ;
  contax:domainOrSubjectIncludes bot:Zone ;
.
bhp:mw-assessmentScore-BPC
  rdf:type owl:DatatypeProperty ;
  dcterms:source <https://www.monumentenwacht.be/> ;
  rdfs:comment """Property to indicate the building physical condition (BPC) of an assessment connected to an assessed object (cp:hasAssessment) according to the methodology of Monumentenwacht Vlaanderen. The value of the property should be a positive integer between 1 and 6. The scale should be interpretted as follows:
1 = excellent
2 = good
3 = fair
4 = average
5 = bad
6 = very bad"""@en ;
  rdfs:isDefinedBy <https://w3id.org/con-tax/properties/bhp> ;
  rdfs:label "building physical condition score (according Monumentenwacht)"@en ;
  rdfs:range xsd:positiveInteger ;
  rdfs:subPropertyOf cp:assessmentScore ;
.
bhp:mw-assessmentScore-RCD
  rdf:type owl:DatatypeProperty ;
  dcterms:source <https://www.monumentenwacht.be/> ;
  rdfs:comment """Property to indicate the risk for consequential damage (in case the owner does not react properly to the detected damages) of an assessment connected to an assessed object (cp:hasAssessment) according to the methodology of Monumentenwacht Vlaanderen. The value of the property should be a positive integer between 1 and 6. The scale should be interpretted as follows:
1 = no risk
2 = low risk
3 = fair risk
4 = considerable risk
5 = high risk
6 = acute risk"""@en ;
  rdfs:isDefinedBy <https://w3id.org/con-tax/properties/bhp> ;
  rdfs:label "risk for consequential damage score (according Monumentenwacht)"@en ;
  rdfs:range xsd:positiveInteger ;
  rdfs:subPropertyOf cp:assessmentScore ;
.
bhp:mw-assessmentScore-maintenance
  rdf:type owl:DatatypeProperty ;
  dcterms:source <https://www.monumentenwacht.be/> ;
  rdfs:comment """Property to indicate the attitude and quality of the current maintenance policies of an assessment connected to an assessed object (cp:hasAssessment) according to the methodology of Monumentenwacht Vlaanderen. The value of the property should be a positive integer between 1 and 6. The scale should be interpretted as follows:
1 = excellent
2 = good
3 = fair
4 = average
5 = bad
6 = very bad"""@en ;
  rdfs:isDefinedBy <https://w3id.org/con-tax/properties/bhp> ;
  rdfs:label "maintenance score (according Monumentenwacht)"@en ;
  rdfs:range xsd:positiveInteger ;
  rdfs:subPropertyOf cp:assessmentScore ;
.
bhp:originalArchitect
  rdf:type owl:ObjectProperty ;
  dcterms:source <https://inventaris.onroerenderfgoed.be/> ;
  rdfs:comment "Property to relate an original architect to a site, building or individual construction component. Famous architects with assigned URIs from the Getty ULAN vocabulary can be used as values for this property. Property definition inspired by the Onroerend Erfgoed Vlaanderen built heritage inventory."@en ;
  rdfs:isDefinedBy <https://w3id.org/con-tax/properties/bhp> ;
  rdfs:label "original architect"@en ;
  rdfs:subPropertyOf bhp:relatedArchitect ;
  contax:domainOrSubjectIncludes bot:Element ;
  contax:domainOrSubjectIncludes bot:Zone ;
  contax:domainOrSubjectIncludes contax:ConstructionComponent ;
.
bhp:originsFromPeriod
  rdf:type owl:ObjectProperty ;
  rdfs:comment "Property to indicate the historical time period a spatial building zone or a construction component originates from. Property definition inspired by interviews with built heritage stakeholders."@en ;
  rdfs:isDefinedBy <https://w3id.org/con-tax/properties/bhp> ;
  rdfs:label "origins from period"@en ;
  rdfs:subPropertyOf contax:property_OP ;
  contax:domainOrSubjectIncludes bot:Element ;
  contax:domainOrSubjectIncludes bot:Zone ;
  contax:domainOrSubjectIncludes contax:ConstructionComponent ;
  contax:rangeOrObjectIncludes <https://id.erfgoed.net/thesauri/dateringen/1195> ;
  contax:rangeOrObjectIncludes <https://id.erfgoed.net/thesauri/dateringen/1196> ;
  contax:rangeOrObjectIncludes <https://id.erfgoed.net/thesauri/dateringen/1223> ;
  contax:rangeOrObjectIncludes <https://id.erfgoed.net/thesauri/dateringen/1227> ;
  contax:rangeOrObjectIncludes <https://id.erfgoed.net/thesauri/dateringen/1236> ;
  contax:rangeOrObjectIncludes <https://id.erfgoed.net/thesauri/dateringen/1237> ;
.
bhp:percentageRoofSafetyHooks
  rdf:type owl:DatatypeProperty ;
  dcterms:source <https://www.monumentenwacht.be/> ;
  rdfs:comment "Quantitative property to indicate the percentage of the roof that is provided with safety hooks for ladders and/or fall protection. Property definition inspired by the Monumentenwacht Vlaanderen databases (MAKSBO and IMACS)."@en ;
  rdfs:isDefinedBy <https://w3id.org/con-tax/properties/bhp> ;
  rdfs:label "% of roof safety hooks"@en ;
  rdfs:subPropertyOf contax:property_DP ;
  contax:domainOrSubjectIncludes <http://pi.pauwel.be/voc/buildingelement#Slab-ROOF> ;
  contax:domainOrSubjectIncludes <https://w3id.org/con-tax/components/aat-arch#300002098> ;
  contax:rangeOrObjectIncludes xsd:decimal ;
.
bhp:percentageRoofSafetyHooksEN517
  rdf:type owl:DatatypeProperty ;
  dcterms:source <https://www.monumentenwacht.be/> ;
  rdfs:comment "Quantitative property to indicate the percentage of the roof that is provided with safety hooks for ladders and/or fall protection that comply with the European standard EN 517. Property definition inspired by the Monumentenwacht Vlaanderen databases (MAKSBO and IMACS)."@en ;
  rdfs:isDefinedBy <https://w3id.org/con-tax/properties/bhp> ;
  rdfs:label "% of roof safety hooks EN 517"@en ;
  rdfs:subPropertyOf bhp:percentageRoofSafetyHooks ;
  contax:domainOrSubjectIncludes <http://pi.pauwel.be/voc/buildingelement#Slab-ROOF> ;
  contax:domainOrSubjectIncludes <https://w3id.org/con-tax/components/aat-arch#300002098> ;
  contax:rangeOrObjectIncludes xsd:decimal ;
.
bhp:relatedArchitect
  rdf:type owl:ObjectProperty ;
  dcterms:source <https://inventaris.onroerenderfgoed.be/> ;
  rdfs:comment "Property to relate an architect to a site, building or individual construction component. Famous architects with assigned URIs from the Getty ULAN vocabulary can be used as values for this property. Specializations of this property can be used to assign the original architect (bhp:originalArchitect) or (recent or historic) restoration architects (bhp:restorationArchitect). Property definition inspired by the Onroerend Erfgoed Vlaanderen built heritage inventory."@en ;
  rdfs:isDefinedBy <https://w3id.org/con-tax/properties/bhp> ;
  rdfs:label "related architect"@en ;
  rdfs:subPropertyOf contax:property_OP ;
  contax:domainOrSubjectIncludes bot:Element ;
  contax:domainOrSubjectIncludes bot:Zone ;
  contax:domainOrSubjectIncludes contax:ConstructionComponent ;
.
bhp:restorationArchitect
  rdf:type owl:ObjectProperty ;
  dcterms:source <https://inventaris.onroerenderfgoed.be/> ;
  rdfs:comment "Property to relate a (recent or historic) restoration architect to a site, building or individual construction component. Famous architects with assigned URIs from the Getty ULAN vocabulary can be used as values for this property. Property definition inspired by the Onroerend Erfgoed Vlaanderen built heritage inventory."@en ;
  rdfs:isDefinedBy <https://w3id.org/con-tax/properties/bhp> ;
  rdfs:label "restoration architect"@en ;
  rdfs:subPropertyOf bhp:relatedArchitect ;
  contax:domainOrSubjectIncludes bot:Element ;
  contax:domainOrSubjectIncludes bot:Zone ;
  contax:domainOrSubjectIncludes contax:ConstructionComponent ;
.
cp:assessmentScore
  rdf:type owl:DatatypeProperty ;
  rdfs:subPropertyOf contax:property_DP ;
.
<https://w3id.org/con-tax/zones/aat-buildings#300004790>
  rdf:type rdfs:Resource ;
.
<https://www.monumentenwacht.be/>
  rdf:type rdfs:Resource ;
.
